src/lowparse/pulse/LowParse.Pulse.Endianness.fst
@@ -1,0 +1,226 @@
+module LowParse.Pulse.Endianness
+open LowParse.Pulse.Util
+include LowParse.Spec.Endianness
+
+module U8 = FStar.UInt8
+module E = LowParse.Endianness
+module SZ = FStar.SizeT
+module S = Pulse.Lib.Slice
+
+inline_for_extraction
+noextract
+let be_to_n_t
+  (#t: Type0)
+  (#tot: nat)
+  (u: uinttype u#0 t tot)
+  (len: nat { len <= tot })
+: Tot Type
+= (x: S.slice U8.t) ->
+  (#pm: perm) ->
+  (#v: Ghost.erased (Seq.seq U8.t)) ->
+  (pos: SZ.t) ->
+  stt t
+    (S.pts_to x #pm v ** pure (
+      SZ.v pos == len /\
+      len <= Seq.length v
+    ))
+    (fun res -> S.pts_to x #pm v ** pure (
+      SZ.v pos == len /\
+      len <= Seq.length v /\
+      u.v res == E.be_to_n (Seq.slice v 0 len)
+    ))
+
+inline_for_extraction
+noextract
+```pulse
+fn be_to_n_0
+  (#t: Type0)
+  (#tot: nat)
+  (u: uinttype t tot)
+: be_to_n_t #t #tot u 0
+= (x: S.slice U8.t)
+  (#pm: perm)
+  (#v: Ghost.erased (Seq.seq U8.t))
+  (pos: SZ.t)
+{
+  E.reveal_be_to_n (Seq.slice (v) 0 0);
+  u.zero
+}
+```
+
+open FStar.Math.Lemmas
+open FStar.Mul
+
+inline_for_extraction
+noextract
+```pulse
+fn be_to_n_1
+  (#t: Type)
+  (#tot: nat)
+  (u: uinttype t tot { tot > 0 })
+: (be_to_n_t #t #tot u 1)
+= (x: S.slice U8.t)
+  (#pm: perm)
+  (#v: Ghost.erased (Seq.seq U8.t))
+  (pos: SZ.t)
+{
+  E.reveal_be_to_n (Seq.slice (v) 0 1);
+  E.reveal_be_to_n (Seq.slice (v) 0 0);
+  let last = S.op_Array_Access x 0sz;
+  (u.from_byte last)
+}
+```
+
+inline_for_extraction
+noextract
+```pulse
+fn be_to_n_S
+  (#t: Type)
+  (#tot: nat)
+  (#u: uinttype t tot)
+  (#len: nat { len + 1 <= tot })
+  (ih: be_to_n_t #t #tot u len)
+: (be_to_n_t #t #tot u (len + 1))
+= (x: S.slice U8.t)
+  (#pm: perm)
+  (#v: Ghost.erased (Seq.seq U8.t))
+  (pos: SZ.t)
+{
+  assert_norm (pow2 8 == 256);
+  E.reveal_be_to_n (Seq.slice (v) 0 (len + 1));
+  E.lemma_be_to_n_is_bounded (Seq.slice (v) 0 len);
+  pow2_le_compat (8 * tot) (8 * (len + 1));
+  pow2_le_compat (8 * (len + 1)) (8 * len);
+  pow2_plus (8 * len) 8;
+  let pos' = pos `SZ.sub` 1sz;
+  let last = S.op_Array_Access x pos';
+  let n = ih x #pm #v pos';
+  let blast = u.from_byte last;
+  u.add blast (u.mul256 n)
+}
+```
+
+// attribute for use with delta_attr
+noextract
+noeq
+type must_reduce = | MustReduce_dummy_do_not_use
+
+[@must_reduce]
+noextract
+let rec mk_be_to_n
+  (#t: Type)
+  (#tot: nat)
+  (u: uinttype t tot)
+  (len: nat {len <= tot})
+: Tot (be_to_n_t u len)
+  (decreases len)
+= if len = 0
+  then be_to_n_0 u
+  else if len = 1
+  then be_to_n_1 u
+  else be_to_n_S (mk_be_to_n u (len - 1))
+
+// Disclaimer: a function of type n_to_be_t is ultimately meant to be called with a buffer of size len, so we do not care about any output bytes beyond position len.
+
+inline_for_extraction
+noextract
+let n_to_be_t
+  (#t: Type0)
+  (#tot: nat)
+  (u: uinttype t tot)
+  (len: nat { len <= tot })
+: Tot Type
+= (n: t) ->
+  (x: S.slice U8.t) ->
+  (#v: Ghost.erased (Seq.seq U8.t)) ->
+  (pos: SZ.t) ->
+  stt unit
+    (S.pts_to x v ** pure (
+      SZ.v pos == len /\
+      len <= Seq.length v /\
+      u.v n < pow2 (8 * len)
+    ))
+    (fun _ -> exists* v' . S.pts_to x v' ** pure (
+      SZ.v pos == len /\
+      len <= Seq.length v /\
+      Seq.length v' == Seq.length v /\
+      u.v n < pow2 (8 * len) /\
+      Seq.slice (v') 0 len `Seq.equal` n_to_be len (u.v n)
+    ))
+
+inline_for_extraction
+noextract
+```pulse
+fn n_to_be_0
+  (#t: Type0)
+  (#tot: nat)
+  (u: uinttype t tot)
+: (n_to_be_t #t #tot u 0)
+= (n: t)
+  (x: S.slice U8.t)
+  (#v: Ghost.erased (Seq.seq U8.t))
+  (pos: SZ.t)
+{
+  E.reveal_be_to_n (Seq.slice (v) 0 0);
+  ()
+}
+```
+
+inline_for_extraction
+noextract
+```pulse
+fn n_to_be_1
+  (#t: Type)
+  (#tot: nat)
+  (u: uinttype t tot { tot > 0 })
+: (n_to_be_t #t #tot u 1)
+= (n: t)
+  (x: S.slice U8.t)
+  (#v: Ghost.erased (Seq.seq U8.t))
+  (pos: SZ.t)
+{
+  E.reveal_n_to_be 1 (u.v n);
+  E.reveal_n_to_be 0 (u.v n / pow2 8);
+  let n' = u.to_byte n;
+  S.op_Array_Assignment x 0sz n'
+}
+```
+
+inline_for_extraction
+noextract
+```pulse
+fn n_to_be_S
+  (#t: Type)
+  (#tot: nat)
+  (#u: uinttype t tot)
+  (#len: nat {len + 1 <= tot})
+  (ih: n_to_be_t #t #tot u len)
+: (n_to_be_t #t #tot u (len + 1))
+= (n: t)
+  (x: S.slice U8.t)
+  (#v: Ghost.erased (Seq.seq U8.t))
+  (pos: SZ.t)
+{
+  reveal_n_to_be (len + 1) (u.v n);
+  let lo = u.to_byte n;
+  let hi = u.div256 n;
+  let pos' = pos `SZ.sub` 1sz;
+  let _ = ih hi x pos';
+  S.op_Array_Assignment x pos' lo
+}
+```
+
+[@must_reduce]
+noextract
+let rec mk_n_to_be
+  (#t: Type)
+  (#tot: nat)
+  (u: uinttype t tot)
+  (len: nat {len <= tot})
+: Tot (n_to_be_t u len)
+  (decreases len)
+= if len = 0
+  then n_to_be_0 u
+  else if len = 1
+  then n_to_be_1 u
+  else n_to_be_S (mk_n_to_be u (len - 1))
